fix: minor style fixes

regmachine.v
@@ -7,38 +7,35 @@ From event_struct Require Import transitionsystem ident rfsfun.
 (* Here we want to obrain big-step semaintics of simple register machine in   *)
 (* terms of fin_exec_event_structures                                         *)
 (* This file contains definition of:                                          *)
-(*             instr == regmachine instructions                               *)
-(*             seqprog == sequence on instructions ie. one thread of program  *)
-(*             parprog == consurent program (contains several threads)        *)
-(*             thrd_state == state of one thread: pair of our place in        *)
-(*               program (ie. line numder) and map from registers to values   *)
-(*             init_state == initial state of one thred : pair of 0 default   *)
-(*               map that maps all registers to default value                 *)
-(*             config == configuration of program: pair of                    *)
-(*               fin_exec_event_strucure corresponding to our program in      *)
-(*               current state and map form elements of this event structure  *)
-(*               to corresponding thread states                               *)
-(*             thrd_sem == if we are in some thread state we can make one     *)
-(*               step in program and obtain side effect (action on shared     *)
-(*               locals) and a new thread state. But if we want to read from  *)
-(*               shared memory, in general we can do it in defferent ways. So *)
-(*               as a read-from-shared-memory-side effect we return Read x __ *)
-(*               ie. read with hole instead of read value. And as a mapping   *) 
-(*               from registers to values we return somehow codded function   *)
-(*               hole                                                         *)
-(*             ltr_thrd_sem == version of thrd_sem as labeled relation        *)
-(*             writes_seq == function that takes local variable x and         *)
-(*               some event structure and returns all events in this event    *)
-(*               structure that are writing in x                              *)
-(*             es_seq == takes event structure `es`, location `x`, predsessor *)
-(*               event `pr` and returns sequence of `es + Read x v`, where v  *)
-(*               runs on all values  `v` that we can read in location `x`     *)
-(*             add_hole == takes `es`, label with hole `l` (look thrd_sem),   *)
-(*               predsessor event `pr` and return seq `es + l` where l runs   *)
-(*               on all labels that can be obtained by filling the hole in `l`*)
-(*             eval_step == takes config `c`, event `pr` and retunrs seq of   *)
-(*               configurations `c'` that can be reach form `c` making a step *)
-(*               in thread state corresponding to `pr` in `c`                 *)
+(*       instr == regmachine instructions                                     *)
+(*     seqprog == sequence on instructions ie. one thread of program          *)
+(*     parprog == consurent program (contains several threads)                *)
+(*  thrd_state == state of one thread: pair of our place in program (ie. line *)
+(*            numder) and map from registers to values                        *)
+(*  init_state == initial state of one thred : pair of 0 default map that     *)
+(*     maps all registers to default value                                    *)
+(*      config == configuration of program: pair of fin_exec_event_strucure   *)
+(*           corresponding to our program in current state and map form       *)
+(*           elements of this event structure to corresponding thread states  *)
+(*  thrd_sem == if we are in some thread state we can make one step in program*)
+(*     and obtain side effect (action on shared locals) and a new thread state*)
+(*     But if we want to read from shared memory, in general we can do it in  *)
+(*     defferent ways. So as a read-from-shared-memory-side effect we return  *)
+(*     Read x __  ie. read with hole instead of read value. And as a mapping  *)
+(*     from registers to values we return somehow codded function hole        *)
+(*  ltr_thrd_sem == version of thrd_sem as labeled relation                   *)
+(*    writes_seq == function that takes local variable x and some event       *)
+(*          structure and returns all events in this event structure that are *)
+(*          writing in x                                                      *)
+(*        es_seq == takes event structure `es`, location `x`, predsessor event*)
+(*          `pr` and returns sequence of `es + Read x v`, where v runs on all *)
+(*           values  `v` that we can read in location `x`                     *)
+(*      add_hole == takes `es`, label with hole `l` (look thrd_sem),          *)
+(*    predsessor event `pr` and return seq `es + l` where l runs on all labels*)
+(*     that can be obtained by filling the hole in `l`                        *)
+(*     eval_step == takes config `c`, event `pr` and retunrs seq of           *)
+(*        configurations `c'` that can be reach form `c` making a step        *)
+(*        in thread state corresponding to `pr` in `c`                        *)
 (******************************************************************************)
 
 Set Implicit Arguments.
@@ -73,13 +70,28 @@ Definition seqprog := seq instr.
 
 Definition parprog := seq seqprog.
 
-Definition thrd_state := (nat * {fsfun reg -> val with inh})%type.
+Record thrd_state := Thrd_state {
+  ip     : nat;
+  regmap : {fsfun reg -> val with inh}
+}.
 
-Definition init_state : thrd_state := (0, [fsfun with inh]).
+Definition eq_thrd_state st st' := 
+  (ip st == ip st') && (regmap st == regmap st').
 
-Record config := Conf {
-  evstr : exec_event_struct;
-  corr  :> {fsfun E -> thrd_state with init_state}
+Lemma eqthrd_stateP : Equality.axiom eq_thrd_state.
+Proof.
+  case=> ?? [?? /=]; rewrite /eq_thrd_state /=.
+  by apply/(equivP andP); split=> [[/eqP->/eqP->]|[->->]]. 
+Qed.
+
+Canonical thrd_state_eqMixin := EqMixin eqthrd_stateP.
+Canonical thrd_state_eqType := Eval hnf in EqType thrd_state thrd_state_eqMixin.
+
+Definition init_state : thrd_state := {| ip := 0; regmap := [fsfun with inh] |}.
+
+Record config := Config {
+  evstr    : exec_event_struct;
+  trhdmap  :> {fsfun E -> thrd_state with init_state}
 }.
 
 Variable p : seqprog.
@@ -88,18 +100,22 @@ Notation nth := (nth (CJmp 0 0)).
 
 Definition thrd_sem (st : thrd_state) :
   (option (@label unit val) * (val -> thrd_state))%type :=
-  let: (ip, map) := st in
-  match nth p ip with
-  | WriteReg v r => (none,             fun _ => 
-                                       (ip.+1, [fsfun map with r |-> v]))
-  | ReadLoc  r x => (some (Read x __), fun v => 
-                                       (ip.+1, [fsfun map with r |-> v]))
-  | WriteLoc v x => (some (Write x v), fun _ => (ip.+1, map))
-  | CJmp     r n => (none,             fun _ => 
-                                       (if map r != inh then n else ip.+1, map))
+  let: {| ip := i; regmap := map |} := st in
+  match nth p i with
+  | WriteReg v r => (none,
+                     fun _ => {| ip     := i.+1;
+                                 regmap := [fsfun map with r |-> v] |})
+  | ReadLoc  r x => (some (Read x __), 
+                     fun v => {| ip := i.+1;
+                                 regmap := [fsfun map with r |-> v] |})
+  | WriteLoc v x => (some (Write x v), 
+                     fun _ => {| ip := i.+1; regmap := map |})
+  | CJmp     r n => (none,             
+                     fun _ => {| ip := if map r != inh then n else i.+1;
+                                 regmap := map |} )
   end.
 
-Definition ltr_thrd_sem (l : option (@label val val)) (st1 st2 : thrd_state) : bool :=
+Definition ltr_thrd_sem (l : option (@label val val)) st1 st2 : bool :=
   match thrd_sem st1, l with
   | (some (Write x v), st), some (Write y u) => [&& x == y, v == u & st inh == st2]
   | (some (Read  x _), st), some (Read  y u) => (x == y) && (st u == st2)
@@ -108,11 +124,11 @@ Definition ltr_thrd_sem (l : option (@label val val)) (st1 st2 : thrd_state) : b
   end.
 
 Variable (es : exec_event_struct).
-Notation dom := (dom es).
-Notation lab    := (lab es).
-Notation ffpred  := (ffpred es).
-Notation ffrf    := (ffrf es).
-Notation fresh := (fresh_seq dom).
+Notation dom      := (dom es).
+Notation lab      := (lab es).
+Notation ffpred   := (ffpred es).
+Notation ffrf     := (ffrf es).
+Notation fresh_id := (fresh_seq dom).
 
 Arguments add_label_of_Nread {_ _ _ _} _ {_}.
 
@@ -124,39 +140,39 @@ Definition wpred (x : loc) (w : E)
 
 Arguments wpred /.
 
-Definition writes_seq x :
-  seq (sig_subType (fun y => (wpred x y) && (y \in dom))) :=
+Definition writes_seq x : seq {y | (wpred x y) && (y \in dom)} :=
   pmap insub dom.
 
-Lemma ws_mem x 
-   (w : sig_subType (fun y => (wpred x y) && (y \in dom))):
-   (eqtype.val w) \in fresh :: dom .
+Lemma ws_mem x (w : {y | (wpred x y) && (y \in dom)}) :
+   (sval w) \in fresh_id :: dom .
 Proof.
   rewrite ?inE.
   by case: w=> /= ? /andP[?->]. 
 Qed.
 
-Lemma ws_wpred x 
-  (w : sig_subType (fun y => (wpred x y) && (y \in dom))):
-  let: wr := eqtype.val w in
+Lemma ws_wpred x (w : {y | (wpred x y) && (y \in dom)}) :
+  let: wr := sval w in
   let: read_lab := Read x (wval (lab wr)) in
-    ((wr == fresh) && ~~ is_read read_lab) ||
-    (lab wr) << read_lab.
+    add_wr wr fresh_id lab read_lab.
 Proof. by case: w=> /= ? /andP[->]. Qed.
 
 (* TODO: filter by consistentcy *)
-Definition es_seq x {pr} (pr_mem : pr \in fresh :: dom) :
+Definition es_seq x {pr} (pr_mem : pr \in fresh_id :: dom) :
  (seq (exec_event_struct * val)) := 
-  map (fun w => 
-   ((add_event 
+  [seq
+    let: wr := sval w in
+    let: read_lab := Read x (wval (lab wr)) in
     (
-      Add pr_mem (@ws_mem x w) (ws_wpred w))),
-      wval (lab (eqtype.val w)))
-    )
-     (writes_seq x).
+      add_event
+        {| add_lb            := read_lab;
+           add_pred_in_dom   := pr_mem;
+           add_write_in_dom  := @ws_mem x w;
+           add_write_consist := ws_wpred w; |},
+      wval (lab (eqtype.val w))
+    ) | w <- (writes_seq x)].
 
 Definition add_hole  
-  (l : @label unit val) {pr} (pr_mem : pr \in fresh :: dom) :
+  (l : @label unit val) {pr} (pr_mem : pr \in fresh_id :: dom) :
   seq (exec_event_struct * val) :=
   match l with
   | Write x v => 
@@ -165,12 +181,14 @@ Definition add_hole
   | _ => [::]
   end.
 
-Definition eval_step (c : config) {pr} (pr_mem : pr \in fresh :: dom) 
+Definition eval_step (c : config) {pr} (pr_mem : pr \in fresh_id :: dom) 
   : seq config :=
   let: (l, cont_st) := thrd_sem (c pr) in
   if l is some l then
-    [seq (Conf x.1 [fsfun c with fresh |-> cont_st x.2]) |
-     x <- (add_hole l pr_mem)]
-  else [:: Conf (evstr c) [fsfun c with pr |-> cont_st inh]].
+    [seq let: (e, v) := x in 
+          (Config e [fsfun c with fresh_id |-> cont_st v]) |
+          x <- (add_hole l pr_mem)]
+  else 
+    [:: Config (evstr c) [fsfun c with pr |-> cont_st inh]].
 
 End RegMachine.
